src/Std/Data/HashMap/Lemmas.lean
@@ -1158,7 +1158,7 @@ theorem all_keys [LawfulHashable α] [EquivBEq α] {p : α → Bool} :
     m.keys.all p = m.all (fun a _ => p a) :=
   DHashMap.Const.all_keys
 
-variable {ρ : Type w} [ForIn Id ρ (α × β)]
+variable {ρ : Type w} [ForIn Id ρ (α × β)] [ForInNew Id ρ (α × β)]
 
 @[simp, grind =]
 theorem insertMany_nil :
@@ -2198,7 +2198,7 @@ end Diff
 -- we do not add `@[grind]` annotations to any of its lemmas.
 
 variable {m : HashMap α Unit}
-variable {ρ : Type w} [ForIn Id ρ α]
+variable {ρ : Type w} [ForIn Id ρ α] [ForInNew Id ρ α]
 
 @[simp]
 theorem insertManyIfNewUnit_nil :
